Fp/EFixedPoint/Basic.lean
@@ -1,0 +1,54 @@
+import Fp.FixedPoint.Basic
+import Fp.Constants.Basic
+
+/--
+A fixed point number extended with infinity and NaN.
+-/
+@[ext]
+structure EFixedPoint (width prec : Nat) where
+  state : State
+  num : FixedPoint width prec
+deriving DecidableEq, Repr
+
+attribute [bv_normalize] EFixedPoint.ext_iff
+
+@[bv_normalize]
+theorem EFixedPoint.ext_iff_beq {x y : EFixedPoint width exOffset}
+  : (x == y) = (x.state == y.state && x.num == y.num) := by
+  cases h : (x == y) <;> simp_all [EFixedPoint.ext_iff]
+
+@[bv_normalize]
+theorem EFixedPoint.bne_to_beq {x y : EFixedPoint width exOffset}
+  : (x != y) = !(x == y) := by
+  cases h : (x != y) <;> simp_all [EFixedPoint.ext_iff]
+
+@[bv_normalize]
+theorem EFixedPoint.eq_cond_state {x y : EFixedPoint width exOffset} :
+  (bif b then x else y).state = bif b then x.state else y.state := by
+  cases b <;> rfl
+
+@[bv_normalize]
+theorem EFixedPoint.eq_cond_num {x y : EFixedPoint width exOffset} :
+  (bif b then x else y).num = bif b then x.num else y.num := by
+  cases b <;> rfl
+
+class HExOffset (e : Nat) (m : Nat) where
+  h : e < m
+
+instance HExOffsetSucc [hex : HExOffset e m] :
+    HExOffset e (m + 1) where
+  h := by
+    have := hex.h
+    omega
+
+instance HExOffsetAdd [hex : HExOffset e m] (k : Nat) :
+    HExOffset (e + k) (m + k) where
+  h := by
+    have := hex.h
+    omega
+
+instance HExOffsetDouble [hex : HExOffset e m] :
+    HExOffset (e + e) (m + m) where
+  h := by
+    have := hex.h
+    omega
