Fp/PackedFloat/Basic.lean
@@ -1,0 +1,48 @@
+/-!
+## Packed Floating Point Numbers
+-/
+
+/--
+A packed floating point number,
+whose exponent and significand width are encoded at the type level.
+-/
+@[ext]
+structure PackedFloat (exWidth sigWidth : Nat) where
+    /-- Sign bit. -/
+    sign : Bool
+    /-- Exponent of the packed float. -/
+    ex : BitVec exWidth
+    /-- Significand (mantissa) of the packed float. -/
+    sig : BitVec sigWidth
+deriving DecidableEq, Repr, Inhabited
+
+attribute [bv_normalize] PackedFloat.ext_iff
+
+@[bv_normalize]
+theorem PackedFloat.ext_iff_beq {x y : PackedFloat exWidth sigWidth}
+  : (x == y) = (x.sign == y.sign && x.ex == y.ex && x.sig == y.sig) := by
+  cases h : (x == y) <;> simp_all [PackedFloat.ext_iff]
+
+@[bv_normalize]
+theorem PackedFloat.bne_to_beq {x y : PackedFloat exWidth sigWidth}
+  : (x != y) = !(x == y) := by
+  cases h : (x != y) <;> simp_all [PackedFloat.ext_iff]
+
+@[bv_normalize]
+theorem PackedFloat.eq_cond_sign {x y : PackedFloat exWidth sigWidth} :
+  (bif b then x else y).sign = bif b then x.sign else y.sign := by
+  cases b <;> rfl
+
+@[bv_normalize]
+theorem PackedFloat.eq_cond_ex {x y : PackedFloat exWidth sigWidth} :
+  (bif b then x else y).ex = bif b then x.ex else y.ex := by
+  cases b <;> rfl
+
+@[bv_normalize]
+theorem PackedFloat.eq_cond_sig {x y : PackedFloat exWidth sigWidth} :
+  (bif b then x else y).sig = bif b then x.sig else y.sig := by
+  cases b <;> rfl
+
+instance : Repr (PackedFloat exWidth sigWidth) where
+  reprPrec x _prec :=
+    f!"\{ sign := {if x.sign then "-" else "+"}, ex := {x.ex}, sig := {x.sig} }"
